IMPminus_TM/TM_GOTO/TM_to_GOTO_on_List.thy
@@ -8,6 +8,9 @@ locale TM_to_GOTO_on_List =
       and G :: nat \<comment>\<open>G: size of tape character set\<close>
   assumes TM: "turing_machine K G M"
 
+    fixes Q :: nat \<comment>\<open>Q: number of states, halting state excluded\<close>
+  assumes Q: "Q = length M"
+
     fixes TPS :: "tape list"  \<comment>\<open>TPS: input tapes\<close>
       and T :: nat            \<comment>\<open>T: runtime\<close>
       and TPS' :: "tape list" \<comment>\<open>TPS': output tapes\<close>
@@ -15,8 +18,6 @@ locale TM_to_GOTO_on_List =
 
     fixes MAX_LEN :: nat    \<comment>\<open>maximum length of all tapes during the execution of the TM\<close>
 begin
-
-definition "Q = length M" \<comment>\<open>Q: number of states, halting state excluded\<close>
 
 subsection \<open>Helper functions\<close>
 
@@ -34,29 +35,77 @@ subsection \<open>Definition of the transform function\<close>
 
 value "List.product [0..<5] (product_lists (replicate 4 [0..1]))"
 
-fun entrance_block_gen :: "(state \<times> symbol list) list \<Rightarrow> pc \<Rightarrow> GOTO\<^sub>l_prog" where
-  "entrance_block_gen [] pc = [
-    IF ST = L [Q] THEN GOTO\<^sub>l pc,
-    TMP 0 ::=\<^sub>l ReadChs [0..<K]]" | (*TODO: replace pc with the label of M_end*)
-  "entrance_block_gen ((q, chs) # q_chs_s) pc =
-    entrance_block_gen q_chs_s (Suc pc) @ [
-    IF ST = L [q] AND TMP 0 = L chs THEN GOTO\<^sub>l pc]" (*TODO: replace pc with the label of M_q_chs*)
+fun entrance_block_gen :: "(state \<times> symbol list) list \<Rightarrow> nat \<Rightarrow> GOTO\<^sub>l_prog" where
+  "entrance_block_gen [] _ = [
+     IF ST = L [Q] THEN GOTO\<^sub>l pc_halt,
+     TMP 0 ::=\<^sub>l ReadChs [0..<K]]" |
+  "entrance_block_gen ((q, chs) # q_chs_s) idx =
+    entrance_block_gen q_chs_s (Suc idx) @ [
+    IF ST = L [q] AND TMP 0 = L chs
+    THEN GOTO\<^sub>l ((Suc (Suc (Q * G ^ MAX_LEN))) + idx * (Suc (3 * K)))]"
+
+lemma entrance_block_gen_length: "length (entrance_block_gen q_xs_s n) = Suc (Suc (length q_xs_s))"
+  by (induction q_xs_s arbitrary: n) auto
 
 definition entrance_block :: "GOTO\<^sub>l_prog" where
   "entrance_block =
    entrance_block_gen (List.product [0..<Q] (product_lists (replicate MAX_LEN [0..<G]))) 0"
 
+lemma entrance_block_length: "length entrance_block = Suc (Suc (Q * G ^ MAX_LEN))"
+proof -
+  have "length [0..<G] = G"
+    by simp
+  then have "map length (replicate MAX_LEN [0..<G]) = replicate MAX_LEN G"
+    by simp
+  moreover
+  have "fold (*) (replicate MAX_LEN G) 1 = G ^ MAX_LEN"
+    using fold_replicate [where ?f = "(*)" and ?n = MAX_LEN and ?x = G]
+    using funpow_times_power [where ?x = G and ?f = "\<lambda>x. MAX_LEN"]
+    by auto
+  moreover
+  have "foldr (*) (replicate MAX_LEN G) 1 = fold (*) (replicate MAX_LEN G) 1"
+    by force
+  ultimately
+  have "length (product_lists (replicate MAX_LEN [0..<G])) = G ^ MAX_LEN"
+    using length_product_lists [of "replicate MAX_LEN [0..<G]"]
+    by simp
+  then have "length (List.product [0..<Q] (product_lists (replicate MAX_LEN [0..<G]))) =
+             Q * G ^ MAX_LEN"
+    by auto
+  then show ?thesis
+    unfolding entrance_block_def
+    using entrance_block_gen_length
+    by fastforce
+qed
+
 fun block_for_q_and_chs :: "state \<times> action list \<Rightarrow> GOTO\<^sub>l_prog" where
-  "block_for_q_and_chs q_act_s = [
-    ST ::=\<^sub>l L [[*] q_act_s]] @
+  "block_for_q_and_chs q_act_s =
+     (ST ::=\<^sub>l L [[*] q_act_s]) # \<comment> \<open>update state\<close>
      (concat (map (\<lambda>n. [
-        TapeModify n (q_act_s [.] n),
+        TapeModify n (q_act_s [.] n), \<comment> \<open>tape modification\<close>
         case q_act_s [~] n of
-          Left \<Rightarrow> MoveLeft n |
-          Right \<Rightarrow> MoveRight n |
-          Stay \<Rightarrow> NOP\<^sub>l,
-        GOTO\<^sub>l 0])
-      [0..<K]))"
+          Left \<Rightarrow> MoveLeft n | Right \<Rightarrow> MoveRight n | Stay \<Rightarrow> NOP\<^sub>l, \<comment> \<open>head movement\<close>
+        GOTO\<^sub>l pc_start])
+      [0..<K]))" \<comment> \<open>for each tape\<close>
+
+lemma length_block_for_q_and_chs: "length (block_for_q_and_chs q_act_s) = Suc (3 * K)"
+proof -
+  let ?f = "(\<lambda>n. [
+    TapeModify n (q_act_s [.] n), \<comment> \<open>tape modification\<close>
+    case q_act_s [~] n of
+      Left \<Rightarrow> MoveLeft n | Right \<Rightarrow> MoveRight n | Stay \<Rightarrow> NOP\<^sub>l, \<comment> \<open>head movement\<close>
+    GOTO\<^sub>l pc_start])"
+  have "length (?f n) = 3" for n by auto
+  then have "map length (map ?f [0..<K]) = replicate K 3"
+    by (simp add: comp_def map_replicate_trivial)
+  moreover
+  have "sum_list (replicate K 3) = 3 * K"
+    by (simp add: sum_list_replicate)
+  ultimately
+  have "length (concat (map ?f [0..<K])) = 3 * K"
+    by (simp add: length_concat)
+  then show ?thesis by auto
+qed
 
 definition blocks_for_actions :: "GOTO\<^sub>l_prog" where
   "blocks_for_actions =
@@ -65,7 +114,7 @@ definition blocks_for_actions :: "GOTO\<^sub>l_prog" where
 
 
 definition GOTO_on_List_Prog :: "GOTO\<^sub>l_prog" where
-  "GOTO_on_List_Prog = entrance_block @ blocks_for_actions @ [HALT\<^sub>l]"
+  "GOTO_on_List_Prog = HALT\<^sub>l # entrance_block @ blocks_for_actions @ [HALT\<^sub>l]"
 
 subsection \<open>Correctness of the transform function\<close>
 
@@ -75,24 +124,6 @@ theorem TM_to_GOTO_on_List_correct:
   sorry
 
 subsection \<open>Runtime of the transformed program\<close>
-
-lemma length_entrance_block_gen: "length (entrance_block_gen l n) = Suc (Suc (length l))"
-  by (induction l arbitrary: n) auto
-
-lemma "length entrance_block = Suc (Suc (Q * (MAX_LEN ^ G)))"
-proof -
-  have "length [0..<Q] = Q" by force
-  moreover
-  have "length (replicate MAX_LEN [0..<G]) = MAX_LEN" by simp
-  have "length (product_lists (replicate MAX_LEN [0..<G])) = MAX_LEN ^ G"
-    sorry
-  have "length (List.product [0..<Q] (product_lists (replicate MAX_LEN [0..<G]))) = Q * (MAX_LEN ^ G)"
-    sorry
-  then show ?thesis
-    unfolding entrance_block_def
-    using length_entrance_block_gen
-    by simp
-qed
 
 theorem TM_to_GOTO_on_List_in_linear_time:
   "\<exists>c. (GOTO_on_List_Prog \<turnstile>\<^sub>l (pc, s) \<rightarrow>\<^bsub>(c * T)\<^esub> (0, s))"
